src/MoreGeneral.v
@@ -4,9 +4,11 @@ Require Import Schemes.
 Require Import SubstSchm.
 Require Import Gen.
 Require Import List.
+Require Import Sublist.
 Require Import ListIds.
 Require Import Context.
 Require Import Typing.
+Require Import Disjoints.
 Require Import NewTypeVariable.
 Require Import SimpleTypes.
 Require Import Subst.
@@ -29,6 +31,352 @@ Inductive more_general_ctx : ctx -> ctx -> Prop :=
 
 Hint Constructors more_general_ctx.
 
+Fixpoint product_list (l1 : list id) (l2 : list ty) :=
+  match l1 with
+  | nil =>  Some nil
+  | st :: l'1 => match l2 with
+                | nil => None
+                | t :: l'2 => match product_list l'1 l'2 with
+                             | None => None
+                             | Some s => Some ((st, t) :: s)
+                             end
+                end
+  end.
+
+Fixpoint ty_from_id_list (l : list id) : list ty :=
+  match l with
+  | nil => nil
+  | x::l' => var x :: ty_from_id_list l'
+  end.
+
+Lemma ty_from_id_list_app : forall l1 l2 : list id,
+    ty_from_id_list (l1 ++ l2) = ty_from_id_list l1 ++ ty_from_id_list l2.
+Admitted.
+
+Hint Resolve ty_from_id_list_app.
+Hint Rewrite ty_from_id_list_app:RE.
+
+Fixpoint map_extend_subst_type (l : list ty) (s2 : substitution) :=
+  match l with
+  | nil => nil
+  | t::l' => apply_subst s2 t :: map_extend_subst_type l' s2
+  end.
+
+Lemma map_extend_app : forall (s : substitution) (l1 l2 : list ty),
+    map_extend_subst_type (l1 ++ l2) s = map_extend_subst_type l1 s ++ map_extend_subst_type l2 s.
+Admitted.
+
+Hint Resolve map_extend_app.
+Hint Rewrite map_extend_app:RE.
+
+Inductive is_prefixe_free2 : list id -> list id -> list id -> Prop :=
+  prefixe_free2_intro : forall C l L : list id,
+    {l1 : list id | L = l ++ l1 /\ are_disjoints C l1} -> is_prefixe_free2 C l L.
+
+Hint Constructors is_prefixe_free2.
+
+Lemma more_general_in_list_FV_schm : forall sigma1 sigma2, more_general sigma1 sigma2 ->
+                                                      forall i, in_list_id i (FV_schm sigma1) = true ->
+                                                           in_list_id i (FV_schm sigma2) = true.
+Proof.
+  induction sigma1; eauto.
+  - intros.
+    induction sigma2; eauto.
+    crush.
+    inverts* H.
+    specialize H1 with (tau:=var i1).
+    edestruct H1.
+    unfold is_schm_instance.
+    exists (nil:inst_subst).
+    reflexivity.
+    simpl in *. inverts* H.
+    crush.
+    inverts* H.
+    specialize H1 with (tau:=con i1).
+    edestruct H1.
+    exists (nil:inst_subst).
+    simpl in *. reflexivity.
+    simpl in *. inverts* H.
+    inverts* H.
+    specialize H1 with (tau:=var i1).
+    simpl in *. crush.
+    edestruct H1.
+Abort.
+
+Fixpoint find_generic_instance (sigma : schm) (tau : ty) :=
+  match sigma with
+  | sc_con i => con i
+  | sc_var i => var i
+  | sc_gen st => tau
+  | sc_arrow sigma1 sigma2 => arrow (find_generic_instance sigma1 tau) (find_generic_instance sigma2 tau)
+  end.
+
+Fixpoint make_constant_gen_subst (n : id) (tau : ty)  :=
+  match n with
+  | O => nil 
+  | S p => tau :: make_constant_gen_subst p tau
+  end.
+Lemma nth_make_constant_gen_subst3 : forall (p n : id) (tau : ty),
+    S n <= p -> nth_error (make_constant_gen_subst p tau) n = Some tau.
+Proof.
+  induction p; crush.
+  destruct n; crush.
+  apply IHp.
+  auto with *.
+Qed.
+
+Hint Resolve nth_make_constant_gen_subst3.
+Hint Rewrite nth_make_constant_gen_subst3:RE.
+
+Lemma apply_subst_inst_make_constant_gen_subst : forall (sigma : schm) (tau : ty) (p : id),
+    max_gen_vars sigma <= p ->
+    apply_inst_subst (make_constant_gen_subst p tau) sigma = Some_schm (find_generic_instance sigma tau).
+Proof.
+  induction sigma; eauto.
+  unfold max_gen_vars.
+  unfold apply_inst_subst.
+  intros tau p le.
+  simpl in le.
+  crush.
+  intros tau p le.
+  simpl.
+  erewrite (IHsigma1 tau p); eauto.
+  erewrite (IHsigma2 tau p); eauto.
+  info_eauto with *.
+  simpl in le.
+  pose proof (PeanoNat.Nat.le_max_l (max_gen_vars sigma1) (max_gen_vars sigma2)).
+  auto with *.
+Qed.
+
+Hint Resolve apply_subst_inst_make_constant_gen_subst.
+Hint Resolve apply_subst_inst_make_constant_gen_subst:RE.
+
+Lemma find_generic_instance_gen_instance_ts : forall (sigma : schm) (tau : ty),
+    is_schm_instance (find_generic_instance sigma tau) sigma.
+Proof.
+  intros.
+  unfold is_schm_instance.
+  exists (make_constant_gen_subst (max_gen_vars sigma) tau).
+  auto.
+Qed.
+
+Hint Resolve find_generic_instance_gen_instance_ts.
+Hint Rewrite find_generic_instance_gen_instance_ts:RE.
+
+Lemma sc_var_more_general_than_sigma : forall (sigma : schm) (st : id),
+    more_general (sc_var st) sigma -> sigma = sc_var st.
+Proof.
+  intros.
+  inversion H. subst.
+  cut (is_schm_instance (find_generic_instance sigma (con 0)) sigma); eauto.
+  intros.
+  cut (is_schm_instance (find_generic_instance sigma (con 0)) (sc_var st)); eauto.
+  intros.
+  inversion_clear H2.
+  destruct sigma; simpl in *.
+  inverts* H3.
+  inverts* H3.
+  inverts* H3.
+  inverts* H3.
+Qed.  
+
+Hint Resolve sc_var_more_general_than_sigma.
+Hint Rewrite sc_var_more_general_than_sigma:RE.
+
+Lemma arrow_sigma_more_general_than_arrow : forall sigma sigma1 sigma2 : schm,
+    (forall tau : ty, is_schm_instance tau sigma -> is_schm_instance tau (sc_arrow sigma1 sigma2)) ->
+    {sig_sig : schm * schm | sigma = sc_arrow (fst sig_sig) (snd sig_sig)}.
+Proof.
+  Admitted.
+
+Hint Resolve arrow_sigma_more_general_than_arrow.
+Hint Resolve arrow_sigma_more_general_than_arrow:RE.
+
+Lemma more_general_arrow_inversion1 : forall sigma1 sigma2 sigma1' sigma2' : schm,
+    more_general (sc_arrow sigma1 sigma2) (sc_arrow sigma1' sigma2') ->
+    more_general sigma1 sigma1'.
+Admitted.
+
+Hint Resolve more_general_arrow_inversion1.
+
+Lemma more_general_arrow_inversion2 : forall sigma1 sigma2 sigma1' sigma2' : schm,
+    more_general (sc_arrow sigma1 sigma2) (sc_arrow sigma1' sigma2') ->
+    more_general sigma2 sigma2'.
+Admitted.
+
+Hint Resolve more_general_arrow_inversion2.
+
+Lemma FV_more_general : forall sigma1 sigma2 : schm, more_general sigma1 sigma2 ->
+                                              is_sublist_id (FV_schm sigma1) (FV_schm sigma2).
+Proof.
+  induction sigma1; crush.
+  apply sc_var_more_general_than_sigma in H.
+  subst. auto.
+  inverts* H.
+  apply arrow_sigma_more_general_than_arrow in H0 as H0'.
+  destruct H0'.
+  subst.
+  simpl.
+  eapply sublist_of_2_app; eauto.
+Qed.
+
+Hint Resolve FV_more_general.
+ 
+Lemma FV_more_general_ctx : forall G1 G2 : ctx, more_general_ctx G1 G2 ->
+                                           Sublist.is_sublist_id (FV_ctx G1) (FV_ctx G2).
+Proof.
+  intros.
+  induction H.
+  - eauto.
+  - simpl.
+    unfold FV_ctx.
+    simpl.
+    fold (FV_ctx G1).
+    fold (FV_ctx G2).
+    eapply sublist_of_2_app;
+    eauto.
+Qed.
+
+Hint Resolve FV_more_general_ctx.
+
+Lemma nth_app : forall (l l1 : list ty) (n : id), n < length l -> nth_error (l ++ l1) n = nth_error l n.
+Admitted.
+
+Hint Resolve nth_app.
+Hint Rewrite nth_app:RE.
+
+Lemma inst_subst_to_subst_aux_4 : forall (G : ctx) (tau1 tau2 : ty) (l L : list id)
+                                   (is_s : list ty) (phi : substitution),
+    are_disjoints (FV_ctx G) l ->
+    apply_inst_subst is_s (fst (gen_ty_aux tau1 G l)) = Some_schm tau2 ->
+    is_prefixe_free2 (FV_ctx G) (snd (gen_ty_aux tau1 G l)) L ->
+    product_list L is_s = Some phi -> apply_subst phi tau1 = tau2.
+Admitted.
+
+Hint Resolve inst_subst_to_subst_aux_4.
+Hint Rewrite inst_subst_to_subst_aux_4:RE.
+
+Lemma nth_map : forall (s : substitution) (x : list ty) (n : id) (tau : ty),
+    nth_error x n = Some tau ->
+    nth_error (map_extend_subst_type x s) n = Some (apply_subst s tau).
+Admitted.
+
+Hint Resolve nth_map.
+Hint Rewrite nth_map:RE.
+
+Lemma index_list_id_nth : forall (l : list id) (v : id) (k : id),
+    index_list_id v l = Some k -> nth_error (ty_from_id_list l) k = Some (var v).
+Admitted.
+
+Hint Resolve index_list_id_nth.
+Hint Rewrite index_list_id_nth:RE.
+
+Lemma length_map : forall (s : substitution) (l : list ty),
+    length (map_extend_subst_type l s) = length l.
+Admitted.
+
+Hint Resolve length_map.
+Hint Rewrite length_map:RE.
+
+Lemma length_ty_from_id_list : forall l : list id, length (ty_from_id_list l) = length l.
+Admitted.
+
+Hint Resolve length_ty_from_id_list.
+Hint Rewrite length_ty_from_id_list:RE.
+
+Lemma index_lt : forall (l : list id) (st : id) (k : id),
+    index_list_id st l = Some k -> k < length l.
+Admitted.
+
+Hint Resolve index_lt.
+
+Lemma nth_app_cons : forall (l : list ty) (tau : ty), nth_error (l ++ tau::nil) (length l) = Some tau.
+simple induction l; auto.
+Qed.
+
+Hint Resolve nth_app_cons.
+
+Lemma length_map2 : forall (s : substitution) (l : list id),
+    length (map_extend_subst_type (ty_from_id_list l) s) = length l.
+Proof.
+  simple induction l; auto.
+  intros; simpl in |- *.
+  rewrite H; auto.
+Qed.
+
+Hint Resolve length_map2.
+Hint Rewrite length_map2:RE.
+
+Lemma length_app_cons : forall (A : Set) (l : list A) (x : A), length (l ++ x :: nil) = S (length l).
+Proof.
+  simple induction l; auto.
+  intros; simpl in |- *; auto.
+Qed.
+
+Hint Resolve length_app_cons.
+Hint Rewrite length_app_cons:RE.
+
+Lemma more_general_gen_type_aux : forall (G1 G2 : ctx) (tau1 tau2 : ty) (phi : substitution)
+                                    (l2 l1 L P : list id) (is_s : inst_subst),
+    more_general_ctx G1 G2 -> are_disjoints (FV_ctx G2) l2 ->
+    are_disjoints (FV_ctx G1) l1 ->
+    apply_inst_subst is_s (fst (gen_ty_aux tau1 G2 l2)) = Some_schm tau2 ->
+    is_prefixe_free2 (FV_ctx G2) (snd (gen_ty_aux tau1 G2 l2)) L ->
+    product_list L is_s = Some phi ->
+    is_prefixe_free2 (FV_ctx G1) (snd (gen_ty_aux tau1 G1 l1)) P ->
+    apply_inst_subst (map_extend_subst_type (ty_from_id_list P) phi)
+                     (fst (gen_ty_aux tau1 G1 l1)) = Some_schm tau2.
+Proof.
+ simple induction tau1.
+ - do 8 intro; intros more_gen_hyp disjoint1 disjoint2.
+   simpl. 
+   cases (in_list_id i (FV_ctx G1)).
+   erewrite (Sublist.sublist_inv1 i (FV_more_general_ctx more_gen_hyp)); eauto.
+   cases (index_list_id i l1).
+   + simpl.
+     intros.
+     inverts* H2.
+     destruct H3.
+     destruct a.
+     rewrite H2.
+     rewrite (ty_from_id_list_app l1 x).
+     rewrite (map_extend_app phi (ty_from_id_list l1) (ty_from_id_list x)).
+     rewrite (nth_app (map_extend_subst_type (ty_from_id_list l1) phi) (map_extend_subst_type (ty_from_id_list x) phi)).
+     erewrite (@nth_map phi (ty_from_id_list l1) i0 (var i)).
+     rewrite (@inst_subst_to_subst_aux_4 G2 (var i) tau2 l2 L is_s phi); eauto.
+     eauto.
+     crush.
+   +
+     intros.
+     inverts* H2.
+     destruct H3.
+     destruct a.
+     rename x into P2.
+     simpl in *.
+     rewrite H2.
+     rewrite (ty_from_id_list_app (l1 ++ i::nil) P2).
+     rewrite (map_extend_app phi (ty_from_id_list (l1 ++ i::nil)) (ty_from_id_list P2)).
+     rewrite (nth_app (map_extend_subst_type (ty_from_id_list (l1 ++ i::nil)) phi)
+             (map_extend_subst_type (ty_from_id_list P2) phi)).
+     erewrite (@nth_map phi (ty_from_id_list (l1 ++ i::nil)) (length l1) (var i)).
+     erewrite (@inst_subst_to_subst_aux_4 G2 (var i) tau2 l2 L is_s phi); eauto.
+     rewrite ty_from_id_list_app; simpl.
+     rewrite <- length_ty_from_id_list; eauto.
+     crush.
+  - 
+
+Lemma more_general_gen_ty : forall (G1 G2 : ctx) (t : ty),
+    more_general_ctx G1 G2 -> more_general (gen_ty t G1) (gen_ty t G2).
+Proof.
+  intros.
+  econstructor. intros.
+  inversion_clear H0.
+  destruct H1.
+  
+Admitted.
+
+Hint Resolve more_general_gen_ty.
+
 Lemma typing_in_a_more_general_ctx : forall (e : term) (G2 G1 : ctx) (t : ty),
     more_general_ctx G1 G2 -> has_type G2 e t -> has_type G1 e t.
 Proof.
@@ -37,17 +385,14 @@ Admitted.
 
 Hint Resolve typing_in_a_more_general_ctx.
 
-Lemma more_general_gen_ty : forall (G1 G2 : ctx) (t : ty),
-    more_general_ctx G1 G2 -> more_general (gen_ty t G1) (gen_ty t G2).
-  (* ultra hard *)
-Admitted.
-
-Hint Resolve more_general_gen_ty.
-
 Lemma more_general_ctx_refl : forall G : ctx, more_general_ctx G G.
 simple induction G; auto.
 intros; elim a; auto.
 Qed.
 
 Hint Resolve more_general_ctx_refl.
- 
+
+Lemma s_gen_t_more_general_than_gen_s_t : forall (s : substitution) (G : ctx) (tau : ty),
+ more_general (apply_subst_schm s (gen_ty tau G)) (gen_ty (apply_subst s tau) (apply_subst_ctx s G)).
+Admitted.
+
